Mostly complete example of delegation to BagADTs.

examples/BookstorewDelegationSemiAutomatic.v
@@ -57,12 +57,12 @@ Definition Order := TupleDef BookStoreSchema sORDERS.
 Definition BookStoreSig : ADTSig :=
   ADTsignature {
       Constructor "Init" : unit -> rep,
-      Method "PlaceOrder" : rep x Order -> rep x bool,
+      (* Method "PlaceOrder" : rep x Order -> rep x bool, *)
       Method "DeleteOrder" : rep x nat -> rep x list Order,
-      Method "AddBook" : rep x Book -> rep x bool,
-      Method "DeleteBook" : rep x nat -> rep x list Book,
-      Method "GetTitles" : rep x string -> rep x list string,
-      Method "NumOrders" : rep x string -> rep x nat
+      (* Method "AddBook" : rep x Book -> rep x bool, *)
+      (* Method "DeleteBook" : rep x nat -> rep x list Book, *)
+      Method "GetTitles" : rep x string -> rep x list string
+      (* Method "NumOrders" : rep x string -> rep x nat *)
     }.
 
 (* Now we write what the methods should actually do. *)
@@ -71,28 +71,28 @@ Definition BookStoreSpec : ADT BookStoreSig :=
   QueryADTRep BookStoreSchema {
     Def Constructor "Init" (_ : unit) : rep := empty,
 
-    update "PlaceOrder" ( o : Order ) : bool :=
-        Insert o into sORDERS,
+    (*update "PlaceOrder" ( o : Order ) : bool :=
+        Insert o into sORDERS, *)
 
     update "DeleteOrder" ( oid : nat ) : list Order :=
         Delete o from sORDERS where o!sISBN = oid ,
 
-    update "AddBook" ( b : Book ) : bool :=
-        Insert b into sBOOKS ,
+    (*update "AddBook" ( b : Book ) : bool :=
+        Insert b into sBOOKS , *)
 
-    update "DeleteBook" ( id : nat ) : list Book :=
-        Delete book from sBOOKS where book!sISBN = id ,
+    (* update "DeleteBook" ( id : nat ) : list Book :=
+        Delete book from sBOOKS where book!sISBN = id , *)
 
     query "GetTitles" ( author : string ) : list string :=
       For (b in sBOOKS)
       Where (author = b!sAUTHOR)
-      Return (b!sTITLE),
+      Return (b!sTITLE)
 
-     query "NumOrders" ( author : string ) : nat :=
+      (* query "NumOrders" ( author : string ) : nat :=
         Count (For (o in sORDERS) (b in sBOOKS)
                Where (author = b!sAUTHOR)
                Where (b!sISBN = o!sISBN)
-               Return ())
+               Return ()) *)
 }.
 
 (* Aliases for internal names of the two tables *)
@@ -127,32 +127,30 @@ Definition OrderStorageDelegate := BagSpec OrderSearchTermMatcher.
 (* In other words, index first on the author field, then the ISBN field.
  * Works especially efficiently for accesses keyed on author. *)
 
-Definition IndexedQueryStructure (qs_schema : QueryStructureSchema)
-  := ilist (fun ns : NamedSchema =>
-                    {matcher : list (@ProperAttribute (schemaHeading (relSchema ns)))
-                                    & Rep (BagSpec (SearchTermFromAttributesMatcher matcher))})
-           (qschemaSchemas qs_schema).
+Definition BookStoreIndices :
+  ilist (fun ns : NamedSchema => list (@ProperAttribute (schemaHeading (relSchema ns))))
+        (qschemaSchemas BookStoreSchema) :=
+  icons _ BookSearchTerm (icons _ OrderSearchTerm (inil _)).
 
-Definition DelegateToBag_AbsR
-           (qs_schema : QueryStructureSchema)
-           (r_o : UnConstrQueryStructure qs_schema)
-           (r_n : IndexedQueryStructure qs_schema)
-  := forall idx,
-       GetUnConstrRelation r_o idx = projT2 (ith_Bounded relName r_n idx).
+Require Import BagsofTuplesADT.
 
-Lemma BookstorewDelegates_AbsR_Pick :
+Definition BookStore_AbsR := (@DelegateToBag_AbsR _ BookStoreIndices).
+
+(* Lemma BookstorewDelegates_AbsR_Pick :
   forall (qs_schema : QueryStructureSchema)
+         indices
          (r_o : UnConstrQueryStructure qs_schema)
-         r_n f,
-    DelegateToBag_AbsR r_o r_n ->
-    refineEquiv {r_n' | DelegateToBag_AbsR (f r_o) r_n} (ret r_o).
+         (r_n : IndexedQueryStructure qs_schema indices),
+    refineEquiv {r_n' | DelegateToBag_AbsR (r_o) r_n} (ret r_o).
 Proof.
   intros r_o; split; intros v Comp_v;
   inversion_by computes_to_inv; subst; unfold BookstorewDelegates_AbsR in *.
   constructor; eauto.
   erewrite ilist_eq;
     [constructor | eauto].
-Qed.
+Qed. *)
+
+Opaque CallBagMethod.
 
 Theorem BookStoreManual :
   Sharpened BookStoreSpec.
@@ -163,235 +161,131 @@ Proof.
   (* First, we unfold various definitions and drop constraints *)
   start honing QueryStructure.
 
-  hone representation using BookstorewDelegates_AbsR.
-
-  hone method "DeleteOrder". {
-
-
-    unfold QSDeletedTuples.
-
-
-
-
-    deleteChecksSucceeded.
-
-    finish honing.
-  }
-
-  (* Then we introduce the BookStore_AbsR abstraction relation *)
   hone representation using BookStore_AbsR.
 
-  (* We start the actual refinement with the constructor, in a fully
-  automated way *)
   hone constructor "Init". {
-    initializer.
+    simplify with monad laws.
+    rewrite refine_QSEmptySpec_Initialize_IndexedQueryStructure.
+    simpl; simplify with monad laws.
+    finish honing.
   }
 
   hone method "DeleteOrder". {
     startMethod BookStore_AbsR.
 
-    deleteChecksSucceeded.
+    match goal with
+        [ H : @DelegateToBag_AbsR ?qs_schema ?indices ?r_o ?r_n
+          |- context[Pick (QSDeletedTuples ?r_o ?idx ?DeletedTuples)] ] =>
+        let dec := constr:(@DecideableEnsembles.dec _ DeletedTuples _) in
+        let storage := eval simpl in (ith_Bounded relName indices idx) in
+        let fs := fields storage in
+        match type of fs with
+        | list (@Attributes ?SC) =>
+          findGoodTerm SC dec ltac:(fun fds tail =>
+            let tail := eval simpl in tail in
+              makeTerm storage fs SC fds tail
+              ltac:(fun tm =>
+                      rewrite (@refine_BagADT_QSDelete_fst _ _ r_o r_n H idx DeletedTuples _ tm)
+                              by prove_extensional_eq))
+      end
+    end.
+
+    simplify with monad laws; cbv beta; simpl.
+
+    match goal with
+        [ H : @DelegateToBag_AbsR ?qs_schema ?indices ?r_o ?r_n
+          |- context[{r_n' | DelegateToBag_AbsR
+                               (UpdateUnConstrRelation ?r_o ?idx
+                                                       (EnsembleDelete (GetUnConstrRelation ?r_o ?idx)
+                                                                       ?DeletedTuples)) r_n'}]] =>
+        let dec := constr:(@DecideableEnsembles.dec _ DeletedTuples _) in
+        let storage := eval simpl in (ith_Bounded relName indices idx) in
+        let fs := fields storage in
+        match type of fs with
+        | list (@Attributes ?SC) =>
+          findGoodTerm SC dec ltac:(fun fds tail =>
+            let tail := eval simpl in tail in
+              makeTerm storage fs SC fds tail
+              ltac:(fun tm =>
+                      let Eqv := fresh in
+                      assert (ExtensionalEq (@DecideableEnsembles.dec (@Tuple SC) DeletedTuples _)
+                                            (SearchTermFromAttributesMatcher storage tm))
+                        as Eqv by prove_extensional_eq;
+                      setoid_rewrite (@refine_BagADT_QSDelete_snd _ _ r_o r_n H idx DeletedTuples _ tm Eqv);
+                      clear Eqv))
+      end
+    end.
+    simplify with monad laws; cbv beta; simpl.
 
     finish honing.
+
   }
 
-  hone method "DeleteBook". {
+   hone method "GetTitles". {
     startMethod BookStore_AbsR.
 
-    setoid_rewrite refine_if_bool_eta.
+    setoid_rewrite refine_Query_In_Enumerate; eauto.
+    setoid_rewrite refine_List_Query_In_Where.
+
+    pose refine_Query_For_In_Find.
+
+    match goal with
+        [ H : @DelegateToBag_AbsR ?qs_schema ?indices ?r_o ?r_n
+          |- context[For (l <- CallBagMethod ?idx {| bindex := "Enumerate"|} ?r_n0 ();
+                          List_Query_In (filter (@DecideableEnsembles.dec _ ?DeletedTuples _) (snd l))
+                                        ?resultComp)]] =>
+        let dec := constr:(@DecideableEnsembles.dec _ DeletedTuples _) in
+        let storage := eval simpl in (ith_Bounded relName indices idx) in
+        let fs := fields storage in
+        match type of fs with
+        | list (@Attributes ?SC) =>
+          findGoodTerm SC dec ltac:(fun fds tail =>
+            let tail := eval simpl in tail in
+              makeTerm storage fs SC fds tail
+                       ltac:(fun tm =>
+                               setoid_rewrite (@refine_Query_For_In_Find _ _ string _ _ H idx dec tm resultComp);
+                      [ | prove_extensional_eq]
+                    ))
+      end
+    end.
     simplify with monad laws.
+    setoid_rewrite ListQueryRefinements.refine_List_Query_In_Return; simplify with monad laws.
+    simpl.
+    setoid_rewrite (refine_pick_val _ H0); simplify with monad laws.
 
-    delete_preserves_primary_keys.
-
-    delete_foreign_key_check_to_Query (sAUTHOR, sISBN).
-
-    Split Constraint Checks;
-      [ deleteChecksSucceeded; reflexivity
-      | deleteChecksFailed].
-  }
-
-  (* We then move on to the "GetTitles" method, which we decide to
-     implement semi-manually *)
-
-  hone method "GetTitles". {
-    (* STEP 1: unfold the definition of the abstraction relation. *)
-    startMethod BookStore_AbsR.
-
-    (* STEP 2: use rewrites to phrase the query in terms of some
-     * concrete list computation. *)
-    (* First, instead of looping over the mathematical relation,
-     * let's loop over an enumeration of the elements in the
-     * concrete data structure. *)
-
-    rewrite refine_List_Query_In by EquivalentBagIsEquivalentIndexedList.
-
-    (* Next, we can implement the [Where] test as a list [filter]. *)
-    rewrite refine_List_Query_In_Where; instantiate (1 := _).
-
-    (* Now the expression is close enough to a list computation, so
-     * we can replace the whole [for] with selection of some list that
-     * is a permutation of the one we're building. *)
-    rewrite refine_List_For_Query_In_Return_Permutation.
-
-    (* A tactic from our library will do this sort of rewriting for us. *)
-    Undo 3.
-    concretize.
-
-    (* STEP 3: more rewrites to find opportunities to use the index
-     * structures efficiently *)
-    (* We are filtering the results of enumerating all entries in a data structure.
-     * There's a method available that combines the two operations. *)
-
-    rewrite filter over BookStorage
-            using search term (Some n, (@None nat, @nil (TSearchTermMatcher BookSchema))).
-
-    (* Again, a generic tactic can handle this phase. *)
-    Undo 1.
-    asPerm BookStorage.
-
-    (* STEP 4: Now we have settled on the final list expression.
-     * Let's commit to using it instead of one of its other permutations. *)
-    setoid_rewrite refine_Permutation_Reflexivity.
-    simplify with monad laws.
-
-    (* As usual, we have automation for this phase. *)
-    Undo 2.
-    commit.
-
-    (* STEP 5: Pick the current database as the new one. *)
-    rewrite refine_pick_val by eauto.
-    simplify with monad laws.
-
-    (* Automated version: *)
-    Undo 2.
-    choose_db BookStore_AbsR.
-
-    (* And we're done! *)
     finish honing.
-  }
-
-  (* We then move on to implementing one of the mutators.
-     Again, we adopt a slightly more manual style to demonstrate the
-     main steps of the implementation. *)
-  hone method "PlaceOrder". {
-
-    (* First, we unfold the definition of our abstraction relation *)
-    startMethod BookStore_AbsR.
-
-    (* Then, we remove trivial or redundant checks *)
-    pruneDuplicates.
-
-    (* Since the specification represents datasets as mathematical
-       sets, every inserted item is paired with a unique ID, which we
-       need to pick. Further refinements will drop this index, which
-       thus doesn't have any computational cost. *)
-
-    pickIndex.
-
-    (* To ease its implementation, we convert this foregin key check
-       into a query *)
-    foreignToQuery.
-
-    (* This query, operating on sets, is then transformed into a
-       filter on lists, making use of the equivalence relations
-       specified by Bookstore_AbsR *)
-    concretize.
-
-    (* At this point, we need to pick a list of results whose elements
-       are a permutation of the one derived from the query. Using
-       permutation-preserving transformations, we substitute slow
-       operations for more efficient ones *)
-    asPerm (BookStorage, OrderStorage).
-
-    (* This representation is reasonably satisfactory; we pick the
-       resulting list, and proceed to a few extra optimizations *)
-    commit.
-
-    (* Now that we have a decision procedure for the constraint checks,
-       all that remains is to proceed to the actual insertions. We
-       distinguish the case where checks succeeded, and the case where
-       checks failed. *)
-    Split Constraint Checks.
-
-    (* First, the case where checks succeed: the insertion is valid: *)
-    checksSucceeded.
-
-    (* Second, the case where checks failed: in that case, the DB
-       remains untouched: *)
-    checksFailed.
-  }
-
-  (* The remaining methods are similar, so we'll just throw the
-   * automation at them. *)
-
-  hone method "AddBook". {
-
-    startMethod BookStore_AbsR.
-
-    (* The, we remove trivial or redundant checks *)
-    pruneDuplicates.
-
-    (* Since the specification represents datasets as mathematical
-       sets, every inserted item is paired with a unique ID, which we
-       need to pick. Further refinements will drop this index, which
-       thus doesn't have any computational cost. *)
-    pickIndex.
-
-    (* To ease its implementation, we convert this functional dependency
-       check into a query *)
-    fundepToQuery.
-
-    (* This query, operating on sets, is then transformed into a
-       filter on lists, making use of the equivalence relations
-       specified by Bookstore_AbsR *)
-    concretize.
-
-    (* At this point, we need to pick a list of results whose elements
-       are a permutation of the one derived from the query. Using
-       permutation-preserving transformations, we substitute slow
-       operations for more efficient ones *)
-    asPerm (BookStorage, OrderStorage).
-
-    (* This representation is reasonnably satisfactory; we pick the
-       resulting list, and proceed to a few extra optimizations *)
-    commit.
-
-    (* Now that we have a decision procedure for the constraint checks,
-       all that remains is to proceed to the actual insertions. We
-       distinguish the case where checks succeeded, and the case where
-       checks failed. *)
-    Split Constraint Checks.
-
-    (* First, the case where checks succeed: the insertion is valid: *)
-
-    checksSucceeded.
-
-    (* Second, the case where checks failed: in that case, the DB
-       remains untouched: *)
-    checksFailed.
-  }
-
-  hone method "NumOrders". {
-    observer.
   }
 
   unfold cast, eq_rect_r, eq_rect, eq_sym; simpl.
 
   (* At this point our implementation is fully computational: we're done! *)
 
-  Show.
+(*
+  FullySharpenEachMethod [BagSig Book (BuildSearchTermFromAttributes BookSearchTerm);
+                           BagSig Order (BuildSearchTermFromAttributes OrderSearchTerm)]
+                         (icons _ (BagSpec (SearchTermFromAttributesMatcher BookSearchTerm))
+                         (icons _ (BagSpec (SearchTermFromAttributesMatcher OrderSearchTerm))
+                                (inil ADT))); simpl;
+  intros; pose (ADTRefinementPreservesMethods (X 1));
+  pose (ADTRefinementPreservesMethods (X 0)); simpl in *.
+  generalize (r1 {| bindex := "Delete" |}).
+  simpl.
+  intros; eapply SharpenIfComputesTo.
+  Show Existentials.
 
-  FullySharpenEachMethod (@nil ADTSig) (inil ADT); simpl;
-  intros.
-
+pose (X 0); simpl in *.
+  generalize (ADTRefinementPreservesConstructors d0).
+  Print refineADT.
+  eapply d0.
   intros; eapply SharpenIfComputesTo; repeat constructor.
   intros; eapply SharpenIfComputesTo; repeat constructor.
-  intros; eapply SharpenIfComputesTo; repeat constructor.
-
+  intros; eapply SharpenIfComputesTo; repeat constructor. 
 Defined.
+*)
+Admitted.
 
-Definition BookStoreImpl : ComputationalADT.cADT BookStoreSig.
+(*Definition BookStoreImpl : ComputationalADT.cADT BookStoreSig.
   extract implementation of BookStoreManual using (inil _).
 Defined.
 
-Print BookStoreImpl.
+Print BookStoreImpl. *)
