src/QueryStructure/Refinements/Bags/BagsofTuplesADT.v
@@ -1,9 +1,302 @@
-Require Export BagsInterface CountingListBags TreeBags Tuple Heading List Program ilist.
+Require Export BagsInterface CountingListBags TreeBags Tuple Heading List Program ilist i2list.
 Require Import String_as_OT IndexedEnsembles DecideableEnsembles.
 Require Import Bool String OrderedTypeEx BagsOfTuples.
 Require Import GeneralQueryRefinements.
 Require Import QueryStructureNotations ListImplementation.
 Require Import AdditionalLemmas AdditionalPermutationLemmas Arith BagADT.
+
+Section BagsOfTuplesRefinements.
+
+  Variable qs_schema : QueryStructureSchema.
+  Definition Bag_index (ns : NamedSchema) :=
+    list (@ProperAttribute (schemaHeading (relSchema ns))).
+
+  Variable indices : ilist Bag_index (qschemaSchemas qs_schema).
+
+  Definition IndexedQueryStructure
+    := i2list (fun ns index => Rep (BagSpec (SearchTermFromAttributesMatcher index))) indices.
+
+  Definition GetIndexedRelation (r_n : IndexedQueryStructure) idx
+    := i2th_Bounded relName r_n idx.
+
+  Definition CallBagMethod idx midx r_n :=
+    Methods (BagSpec (SearchTermFromAttributesMatcher (ith_Bounded relName indices idx))) midx
+            (GetIndexedRelation r_n idx).
+
+  Definition DelegateToBag_AbsR
+             (r_o : UnConstrQueryStructure qs_schema)
+             (r_n : IndexedQueryStructure)
+    := forall idx, GetUnConstrRelation r_o idx = GetIndexedRelation r_n idx.
+
+  Fixpoint Initialize_IndexedQueryStructure
+          (ns : list NamedSchema)
+          (indices' : ilist Bag_index ns)
+          {struct indices'}
+  : Comp (i2list (fun ns index => Rep (BagSpec (SearchTermFromAttributesMatcher index))) indices')
+    := match indices' return Comp (i2list _ indices') with
+      | inil => ret (i2nil _ _)
+      | icons ns ns' index indices'' =>
+        c <- (Constructors
+                (BagSpec (SearchTermFromAttributesMatcher index)) {|bindex := "EmptyBag" |} tt);
+          cs <- (@Initialize_IndexedQueryStructure ns' indices'');
+          ret (i2cons ns index c cs)
+
+    end.
+
+  Lemma refine_QSEmptySpec_Initialize_IndexedQueryStructure
+        : refine {nr' | DelegateToBag_AbsR (DropQSConstraints (QSEmptySpec qs_schema)) nr'}
+                 (Initialize_IndexedQueryStructure indices).
+  Proof.
+    intros v Comp_v.
+    econstructor.
+    unfold IndexedQueryStructure, DelegateToBag_AbsR, GetIndexedRelation.
+  Admitted.
+
+  Definition UpdateIndexedRelation (r_n : IndexedQueryStructure) idx newRel
+  : IndexedQueryStructure :=
+    replace_BoundedIndex2 relName r_n idx newRel.
+
+  Lemma get_update_indexed_eq :
+    forall (r_n : IndexedQueryStructure) idx newRel,
+      GetIndexedRelation (UpdateIndexedRelation r_n idx newRel) idx = newRel.
+  Proof.
+    unfold UpdateIndexedRelation, GetIndexedRelation;
+    intros; simpl; rewrite i2th_replace_BoundIndex_eq; eauto using string_dec.
+  Qed.
+
+  Lemma get_update_indexed_neq :
+    forall (r_n : IndexedQueryStructure) idx idx' newRel,
+      idx <> idx'
+      -> GetIndexedRelation (UpdateIndexedRelation r_n idx newRel) idx' =
+      GetIndexedRelation r_n idx'.
+  Proof.
+    unfold UpdateIndexedRelation, GetIndexedRelation;
+    intros; simpl; rewrite i2th_replace_BoundIndex_neq; eauto using string_dec.
+  Qed.
+
+  Lemma refine_Query_In_Enumerate
+        (ResultT : Type) :
+    forall r_o r_n,
+      DelegateToBag_AbsR r_o r_n
+      -> forall (idx : BoundedString)
+                (resultComp : Tuple -> Comp (list ResultT)),
+           refine (UnConstrQuery_In r_o idx resultComp)
+                  (l <- CallBagMethod idx {|bindex := "Enumerate" |} r_n ();
+                   List_Query_In (snd l) resultComp).
+  Proof.
+    unfold UnConstrQuery_In, QueryResultComp, CallBagMethod;
+    intros; simpl.
+    setoid_rewrite refineEquiv_bind_bind;
+      setoid_rewrite refineEquiv_bind_unit; simpl.
+    unfold List_Query_In.
+    intros v Comp_v; inversion_by computes_to_inv;
+    unfold EnsembleIndexedListEquivalence,
+    UnIndexedEnsembleListEquivalence in *.
+    intuition; destruct_ex; intuition; subst.
+    econstructor; eauto.
+    econstructor; rewrite (H idx); eauto.
+  Qed.
+
+  Lemma flatten_CompList_app_inv
+        {A : Type}
+  : forall (l l' : list (Comp (list A))) v,
+      flatten_CompList (l ++ l') ↝ v
+      -> exists e e',
+           v = app e e'
+           /\ flatten_CompList l ↝ e
+           /\ flatten_CompList l' ↝ e'.
+  Proof.
+    induction l; simpl; intros.
+    - eexists []; exists v; simpl; intuition.
+    - inversion_by computes_to_inv; subst.
+      destruct (IHl _ _ H1) as [e [e' [v_eq [Comp_l Comp_l']]]].
+      rewrite v_eq.
+      exists (app x e); exists e'; intuition.
+      repeat econstructor; eauto.
+  Qed.
+
+  Lemma refine_Join_Query_In_Enumerate'
+        heading
+        (ResultT : Type) :
+    forall r_o r_n,
+      DelegateToBag_AbsR r_o r_n ->
+      forall (idx : BoundedString)
+             (resultComp : Tuple -> Tuple -> Comp (list ResultT))
+             l,
+        refine (List_Query_In l (fun tup : @Tuple heading =>
+                                   UnConstrQuery_In r_o idx (resultComp tup)))
+               (l' <- CallBagMethod idx {|bindex := "Enumerate" |} r_n ();
+                List_Query_In (Join_Lists l (snd l'))
+                              (fun tup_pair => (resultComp (fst tup_pair) (snd tup_pair)))).
+  Proof.
+    intros.
+    unfold List_Query_In; induction l; simpl.
+    - intros v Comp_v; inversion_by computes_to_inv; subst; constructor.
+    - setoid_rewrite IHl; rewrite refine_Query_In_Enumerate; eauto.
+      unfold List_Query_In.
+      setoid_rewrite refineEquiv_bind_bind at 1.
+      setoid_rewrite refineEquiv_bind_bind at 2.
+      intros v Comp_v; inversion_by computes_to_inv.
+      rewrite map_app, map_map in H2; simpl in *.
+      econstructor; eauto.
+      apply flatten_CompList_app_inv in H2; destruct_ex; intuition.
+      subst; repeat (econstructor; eauto).
+  Qed.
+
+  Corollary refine_Join_Query_In_Enumerate
+        (ResultT : Type) :
+    forall r_o r_n,
+      DelegateToBag_AbsR r_o r_n ->
+      forall (idx idx' : BoundedString)
+             (resultComp : Tuple -> Tuple -> Comp (list ResultT)),
+        refine (l <- CallBagMethod idx {|bindex := "Enumerate" |} r_n ();
+                List_Query_In (snd l) (fun tup : Tuple =>
+                                          UnConstrQuery_In r_o idx' (resultComp tup)))
+               (l <- CallBagMethod idx {|bindex := "Enumerate" |} r_n ();
+                l' <- CallBagMethod idx' {|bindex := "Enumerate" |} r_n ();
+                List_Query_In (Join_Lists (snd l) (snd l'))
+                              (fun tup_pair => (resultComp (fst tup_pair) (snd tup_pair)))).
+  Proof.
+    intros.
+    f_equiv; simpl; intro.
+    apply refine_Join_Query_In_Enumerate'; eauto.
+  Qed.
+
+  Lemma refine_Join_Enumerate_Swap
+        (A B ResultT : Type) :
+    forall (c : Comp A) (c' : Comp B)
+           (resultComp : _ -> _ -> Comp (list ResultT)),
+      refineEquiv (For (l <- c;
+                   l' <- c';
+                   resultComp l l'))
+                (For (l' <- c';
+                      l <- c;
+                      resultComp l l')).
+  Proof.
+    split; simpl; intros; f_equiv; intros v Comp_v;
+    inversion_by computes_to_inv; subst;
+    repeat (econstructor; eauto).
+  Qed.
+
+  Local Transparent Query_For.
+
+  Lemma refine_Query_For_In_Find
+        (ResultT : Type)
+  : forall r_o r_n,
+      DelegateToBag_AbsR r_o r_n
+      ->
+      forall (idx : @BoundedString (map relName (qschemaSchemas qs_schema)))
+             filter_dec
+             search_pattern
+             (resultComp : Tuple -> Comp (list ResultT)),
+        ExtensionalEq filter_dec
+                      (SearchTermFromAttributesMatcher
+                         (ith_Bounded relName indices idx) search_pattern)
+        -> refine (For (l <- CallBagMethod idx {|bindex := "Enumerate" |} r_n ();
+                        List_Query_In (filter filter_dec (snd l)) resultComp))
+                  (l <- CallBagMethod idx {|bindex := "Find" |} r_n search_pattern;
+                   List_Query_In (snd l) resultComp).
+  Proof.
+    unfold UnConstrQuery_In, QueryResultComp, CallBagMethod, Query_For;
+    intros; simpl.
+    simplify with monad laws.
+    setoid_rewrite refineEquiv_bind_bind;
+      setoid_rewrite refineEquiv_bind_unit; simpl; f_equiv; intro.
+    unfold List_Query_In.
+    rewrite (filter_by_equiv _ _ H0).
+    intros v Comp_v; econstructor; eauto.
+  Qed.
+
+  Lemma refine_Join_Lists_Where_snd
+        (ResultT : Type) :
+    forall r_n idx idx'
+           (DT : Ensemble Tuple)
+           (DT_Dec : DecideableEnsemble DT)
+           search_pattern
+           (resultComp : Tuple -> Tuple -> Comp (list ResultT)),
+      ExtensionalEq (@dec _ _ DT_Dec)
+                    (SearchTermFromAttributesMatcher
+                       (ith_Bounded relName indices idx') search_pattern)
+      -> refine (For (l <- CallBagMethod idx {| bindex := "Enumerate" |} r_n ();
+                      l' <- CallBagMethod idx' {| bindex := "Enumerate" |} r_n ();
+                      List_Query_In (Join_Lists (snd l) (snd l'))
+                                    (fun tup_pair : Tuple * Tuple =>
+                                       Where (DT (snd tup_pair))
+                                             (resultComp (fst tup_pair) (snd tup_pair)))))
+
+                (For (l <- CallBagMethod idx {| bindex := "Enumerate" |} r_n ();
+                      l' <- CallBagMethod idx' {| bindex := "Find" |} r_n search_pattern;
+                      List_Query_In (Join_Lists (snd l) (snd l'))
+                                    (fun tup_pair : Tuple * Tuple =>
+                                       (resultComp (fst tup_pair) (snd tup_pair))))).
+  Proof.
+    intros; repeat f_equiv; simpl; intro.
+    setoid_rewrite refine_List_Query_In_Where with
+    (P := fun tup_pair => DT (snd tup_pair)).
+  Admitted.
+
+  Lemma refine_List_Query_In_Return
+        (ResultT : Type) :
+    forall l,
+      refine (List_Query_In l (@Query_Return ResultT) ) (ret l).
+  Proof.
+    unfold List_Query_In; induction l; simpl.
+    - reflexivity.
+    - simplify with monad laws; rewrite IHl; simplify with monad laws;
+      reflexivity.
+  Qed.
+
+  Require Import GeneralDeleteRefinements.
+
+  Lemma refine_BagADT_QSDelete_fst :
+    forall r_o r_n,
+      DelegateToBag_AbsR r_o r_n
+      -> forall (idx : @BoundedString (map relName (qschemaSchemas qs_schema)))
+                (DT : Ensemble Tuple)
+                (DT_Dec : DecideableEnsemble DT)
+                search_pattern,
+           ExtensionalEq (@dec _ _ DT_Dec)
+                         (SearchTermFromAttributesMatcher
+                            (ith_Bounded relName indices idx) search_pattern)
+           -> refine {x : list Tuple |
+                      QSDeletedTuples r_o idx DT x}
+                     (l <- (CallBagMethod idx {|bindex := "Delete" |} r_n search_pattern);
+                      ret (snd l)).
+  Proof.
+      intros; setoid_rewrite DeletedTuplesFor; auto.
+      rewrite refine_Query_In_Enumerate by eauto.
+      setoid_rewrite refine_List_Query_In_Where.
+      rewrite (refine_Query_For_In_Find H Query_Return H0).
+      setoid_rewrite refine_List_Query_In_Return.
+      unfold CallBagMethod; simpl; simplify with monad laws;
+      setoid_rewrite refineEquiv_bind_bind;
+      setoid_rewrite refineEquiv_bind_unit; simpl;
+      f_equiv; intro.
+    Qed.
+
+  Lemma refine_BagADT_QSDelete_snd :
+    forall r_o r_n,
+      DelegateToBag_AbsR r_o r_n
+      -> forall (idx : @BoundedString (map relName (qschemaSchemas qs_schema)))
+                (DT : Ensemble Tuple)
+                (DT_Dec : DecideableEnsemble DT)
+                search_pattern,
+           ExtensionalEq (@dec _ _ DT_Dec)
+                         (SearchTermFromAttributesMatcher
+                            (ith_Bounded relName indices idx) search_pattern)
+           -> refine
+                {r_n' |
+                 DelegateToBag_AbsR
+                   (UpdateUnConstrRelation r_o idx (EnsembleDelete
+                                                      (GetUnConstrRelation r_o idx)
+                                                      DT)) r_n'}
+                (l <- (CallBagMethod idx {|bindex := "Delete" |} r_n search_pattern);
+                 ret (UpdateIndexedRelation r_n idx (fst l))).
+  Proof.
+  Admitted.
+
+
+End BagsOfTuplesRefinements.
 
 Section SharpenedBag.
 
@@ -112,7 +405,7 @@ Section SharpenedBag.
          (fun r_o r_n =>
             r_o ≃ benumerate (Bag := BagPlus) r_n
             /\ RepInvPlus r_n).
-    hone constructor "EmptyCache".
+    hone constructor "EmptyBag".
     {
       simplify with monad laws.
       refine pick val bempty.
@@ -190,10 +483,6 @@ Section SharpenedBag.
       eapply Permutation_EnsembleIndexedListEquivalence; simpl; eauto.
     }
 
-    hone method "Update".
-    {
-    }
-
     FullySharpenEachMethod (@nil ADTSig) (inil ADT); simpl.
 
   Defined.
@@ -203,3 +492,6 @@ Section SharpenedBag.
   Defined.
 
 End SharpenedBag.
+
+Opaque CallBagMethod.
+Arguments CallBagMethod : simpl never.
